# nth-number
Yes, now we have the formula for the sequence.

Given the initial terms:
ğ‘›1=1
n2=2
n3=3
n4=4

For ğ‘›â‰¥5
nâ‰¥5, the formula for the ğ‘›
n-th term is:
n(k)=n(kâˆ’1)+n(kâˆ’2)+n(kâˆ’3)+n(kâˆ’4)
 
This means each term from the 5th onward is the sum of the previous four terms. For example:

n5=n1+n2+n3+n4=10
ğ‘›6=ğ‘›2+ğ‘›3+ğ‘›4+ğ‘›5=19

You can now use this recurrence relation to calculate any term in the sequence!

How to run:
Java:
Compile: javac Sequence.java
Run: java Sequence
C:
Compile: gcc -o sequence sequence.c
Run: ./sequence
